zoo_saturn/inf_ws_queue_1: Rewrite.

theories/zoo_saturn/inf_ws_queue_1.v
@@ -117,6 +117,7 @@ Section inf_ws_queue_1_G.
     metadata_history : gname ;
     metadata_winner : gname ;
   }.
+  Implicit Types γ : metadata.
 
   #[local] Instance metadata_eq_dec : EqDecision metadata :=
     ltac:(solve_decision).
@@ -185,7 +186,7 @@ Section inf_ws_queue_1_G.
       Hwinner_steal{_{}}
     )".
 
-  #[local] Definition au γ front P : iProp Σ :=
+  #[local] Definition winner_au γ front P : iProp Σ :=
     AU <{
       ∃∃ vs,
       model₁ γ vs
@@ -197,16 +198,31 @@ Section inf_ws_queue_1_G.
     , COMM
       P
     }>.
-
-  #[local] Definition winner_model γ id front P : iProp Σ :=
-    identifier_model' id ∗
+  #[local] Definition winner_pending_1 γ front P id : iProp Σ :=
     winner_steal γ front P ∗
-    au γ front P.
-  #[local] Instance : CustomIpatFormat "winner_model" :=
+    identifier_model' id ∗
+    winner_au γ front P.
+  #[local] Instance : CustomIpatFormat "winner_pending_1" :=
     "(
-      Hid{_{!}} &
       Hwinner_steal{_{!}} &
-      HP
+      Hid{_{!}} &
+      HP{}
+    )".
+  #[local] Definition winner_pending_2 γ front id : iProp Σ :=
+    ∃ P,
+    winner_pending_1 γ front P id.
+  #[local] Instance : CustomIpatFormat "winner_pending_2" :=
+    "(
+      %P{} &
+      (:winner_pending_1 {//} {/!/})
+    )".
+  #[local] Definition winner_linearized γ front P : iProp Σ :=
+    winner_steal γ front P ∗
+    P.
+  #[local] Instance : CustomIpatFormat "winner_linearized" :=
+    "(
+      Hwinner_steal{_{!}} &
+      HP{}
     )".
 
   #[local] Definition inv_state_empty γ stable front back hist lhist : iProp Σ :=
@@ -238,8 +254,7 @@ Section inf_ws_queue_1_G.
       | [] =>
           False
       | id :: _ =>
-          ∃ P,
-          winner_model γ id front P
+          winner_pending_2 γ front id
       end
     ).
   #[local] Instance : CustomIpatFormat "inv_state_nonempty" :=
@@ -264,7 +279,7 @@ Section inf_ws_queue_1_G.
     | [] =>
         False
     | id :: _ =>
-        winner_model γ id front P
+        winner_pending_1 γ front P id
     end.
   #[local] Instance : CustomIpatFormat "inv_state_nonempty_steal" :=
     "(
@@ -277,7 +292,7 @@ Section inf_ws_queue_1_G.
       {>;}% &
       {>;}-> &
       {>;}%Hhist{} &
-      (:winner_model)
+      (:winner_pending_1)
     )".
   #[local] Definition inv_state_emptyish γ stable front back hist lhist : iProp Σ :=
     ∃ P,
@@ -286,8 +301,7 @@ Section inf_ws_queue_1_G.
     ⌜lhist = hist⌝ ∗
     ⌜length hist = S front⌝ ∗
     ( winner_pop γ front P
-    ∨ winner_steal γ front P ∗
-      P
+    ∨ winner_linearized γ front P
     ).
   #[local] Instance : CustomIpatFormat "inv_state_emptyish" :=
     "(
@@ -327,8 +341,7 @@ Section inf_ws_queue_1_G.
     ⌜front = back⌝ ∗
     ⌜lhist = hist⌝ ∗
     ⌜length hist = S front⌝ ∗
-    winner_steal γ front P ∗
-    P.
+    winner_linearized γ front P.
   #[local] Instance : CustomIpatFormat "inv_state_emptyish_steal" :=
     "(
       { {lazy}{>}%Hstate{}
@@ -340,8 +353,7 @@ Section inf_ws_queue_1_G.
       {>;}-> &
       {>;}-> &
       {>;}%Hhist{} &
-      Hwinner_steal &
-      HP
+      (:winner_linearized)
     )".
   #[local] Definition inv_state_superempty γ stable front back hist lhist : iProp Σ :=
     ⌜stable = Unstable⌝ ∗
@@ -857,11 +869,11 @@ Section inf_ws_queue_1_G.
       iDestruct "Hwinner" as "[(:winner =3) | Hwinner]".
       + iDestruct (winner_pop_exclusive with "Hwinner_pop Hwinner_pop_3") as %[].
       + destruct prophs as [| id prophs]; first done.
-        iDestruct "Hwinner" as "(%P_ & (:winner_model))".
+        iDestruct "Hwinner" as "(:winner_pending_2 =_)".
         iDestruct (winner_agree with "Hwinner_pop Hwinner_steal") as "#(<- & $)".
         iSteps.
     - iDestruct "Hstate" as "(:inv_state_emptyish)".
-      iDestruct "Hwinner" as "[Hwinner_pop_ | (Hwinner_steal & HP)]".
+      iDestruct "Hwinner" as "[Hwinner_pop_ | (:winner_linearized)]".
       + iDestruct (winner_pop_exclusive with "Hwinner_pop Hwinner_pop_") as %[].
       + iDestruct (winner_agree with "Hwinner_pop Hwinner_steal") as "#(<- & $)".
         iSteps.
@@ -887,11 +899,11 @@ Section inf_ws_queue_1_G.
       destruct prophs as [| id prophs].
       + iDestruct "Hwinner" as "[(:winner =3) | []]".
         iDestruct (winner_steal_exclusive with "Hwinner_steal Hwinner_steal_3") as %[].
-      + iDestruct "Hwinner" as "[(:winner =3) | (%P_ & (:winner_model !=))]".
+      + iDestruct "Hwinner" as "[(:winner =3) | (:winner_pending_2 =_ !=)]".
         * iDestruct (winner_steal_exclusive with "Hwinner_steal Hwinner_steal_3") as %[].
         * iDestruct (winner_steal_exclusive with "Hwinner_steal Hwinner_steal_") as %[].
     - iDestruct "Hstate" as "(:inv_state_emptyish)".
-      iDestruct "Hwinner" as "[Hwinner_pop | (Hwinner_steal_ & _)]".
+      iDestruct "Hwinner" as "[Hwinner_pop | (:winner_linearized !=)]".
       + iDestruct (winner_agree with "Hwinner_pop Hwinner_steal") as "#(<- & $)".
         iSteps.
       + iDestruct (winner_steal_exclusive with "Hwinner_steal Hwinner_steal_") as %[].
@@ -1547,7 +1559,7 @@ Section inf_ws_queue_1_G.
 
     iDestruct (inv_state_Nonempty with "Hstate") as %->; first done.
     iDestruct "Hstate" as "(:inv_state_nonempty =2)".
-    iDestruct "Hwinner" as "[(:winner) | (%P & (:winner_model !=))]"; last first.
+    iDestruct "Hwinner" as "[(:winner) | (:winner_pending_2 !=)]"; last first.
     { iDestruct (identifier_model_exclusive with "Hid Hid_") as %[]. }
 
     destruct vs2 as [| v vs2]; first naive_solver lia.
@@ -1556,8 +1568,8 @@ Section inf_ws_queue_1_G.
 
     iSplitR "Hwinner_pop".
     { iExists Nonempty. iFrameSteps.
-      rewrite Hbranch3. iSteps. iIntros "!> !>".
-      rewrite /au. iAuIntro.
+      rewrite Hbranch3 /winner_pending_2. iSteps. iIntros "!> !>".
+      rewrite /winner_au. iAuIntro.
       iApply (aacc_aupd_commit with "HΦ"); first done. iIntros "%vs (:model)". injection Heq as <-.
       iDestruct (meta_agree with "Hmeta Hmeta_") as %<-. iClear "Hmeta_".
       iAaccIntro with "Hmodel₁"; first iSteps. iIntros "%v_ %vs' (-> & Hmodel₁ & Hhistory_at_) !>".
@@ -1768,7 +1780,7 @@ Section inf_ws_queue_1_G.
       destruct (decide (head $ prophss1 front1 = Some id)) as [(prophs0 & Hprophss1)%head_Some | Hbranch2].
 
       + rewrite Hprophss1.
-        iDestruct "Hwinner" as "[(:winner) | (%P & (:winner_model !=))]"; last first.
+        iDestruct "Hwinner" as "[(:winner) | (:winner_pending_2 !=)]"; last first.
         { iDestruct (identifier_model_exclusive with "Hid Hid_") as %[]. }
         iMod (winner_update front1 inhabitant with "Hwinner_pop Hwinner_steal") as "(Hwinner_pop & Hwinner_steal)".
 
@@ -1810,7 +1822,7 @@ Section inf_ws_queue_1_G.
         iDestruct (wise_prophets_full_get _ front1 with "Hprophet_model") as "#Hprophet_full".
         iEval (rewrite Hpasts1 //=) in "Hprophet_full".
         destruct (prophss1 front1) as [| id_winner prophs]; first done.
-        iDestruct "Hwinner" as "(%P & (:winner_model !=))".
+        iDestruct "Hwinner" as "(:winner_pending_2 !=)".
 
         iMod "HP" as "(%vs & Hmodel₁ & _ & HP)".
         iDestruct (model_agree with "Hmodel₁ Hmodel₂") as %->.
